hol/p4_exec_semScript.sml
@@ -2363,6 +2363,41 @@ End
 (*  Frame list semantics  *)
 (**************************)
 
+Definition scopes_to_pass_exec_def:
+ scopes_to_pass_exec (funn:funn) (func_map_g:func_map) (b_func_map:b_func_map) (g_scope_list:g_scope_list) =
+  case g_scope_list of
+  | [block_scope; global_scope] =>
+   (case funn of
+    | (funn_name x) =>
+     (case ALOOKUP b_func_map x of
+      | SOME (stmt, x_d_l) => SOME [block_scope; global_scope]
+      | NONE =>
+       (case ALOOKUP func_map_g x of
+        | SOME (stmt, x_d_l) => SOME ([[]; global_scope])
+        | NONE => SOME [block_scope; global_scope]))
+    | _ => SOME ([[]; global_scope]))
+  | _ => NONE
+End
+
+Definition scopes_to_retrieve_exec_def:
+ scopes_to_retrieve_exec (funn:funn) (func_map_g:func_map) (b_func_map:b_func_map) (g_scope_list_og:g_scope_list) (g_scope_list:g_scope_list) =
+  case g_scope_list_og of
+   | [block_scope_og; global_scope_og] =>
+    (case g_scope_list of
+     | [block_scope; global_scope] =>
+      (case funn of
+       | (funn_name x) =>
+        (case ALOOKUP b_func_map x of
+         | SOME (stmt, x_d_l) => SOME [block_scope; global_scope]
+         | NONE =>
+          (case ALOOKUP func_map_g x of
+           | SOME (stmt, x_d_l) => SOME [block_scope_og; global_scope]
+           | NONE => SOME [block_scope; global_scope]))
+       | _ => SOME [block_scope_og; global_scope])
+     | _ => NONE)
+   | _ => NONE
+End
+
 Definition frames_exec_def:
  (******************************************)
  (* Catch-all clauses for special statuses *)
@@ -2376,7 +2411,7 @@ Definition frames_exec_def:
  (*********)
  (* Comp2 + Comp1 case of multiple frames *)
  (frames_exec uninit (apply_table_f, ext_map, func_map, b_func_map, pars_map, tbl_map) (ascope, g_scope_list, ((funn, stmt_stack, scope_list)::((funn', stmt_stack', scope_list')::frame_list'')), status_running) =
-  (case scopes_to_pass funn func_map b_func_map g_scope_list of
+  (case scopes_to_pass_exec funn func_map b_func_map g_scope_list of
    | SOME g_scope_list' =>
     (case map_to_pass funn b_func_map of
      | SOME b_func_map' =>
@@ -2391,15 +2426,15 @@ Definition frames_exec_def:
              | [(funn, stmt_stack'', scope_list'')] =>
               (case assign g_scope_list'' v (lval_varname (varn_star funn)) of
                | SOME g_scope_list''' =>
-                (case scopes_to_retrieve funn func_map b_func_map g_scope_list g_scope_list''' of
+                (case scopes_to_retrieve_exec funn func_map b_func_map g_scope_list g_scope_list''' of
                  | SOME g_scope_list'''' =>
                   (case lookup_funn_sig_body funn func_map b_func_map ext_map of
                    | SOME (stmt'', x_d_l) =>
-                    (case scopes_to_pass funn' func_map b_func_map g_scope_list'''' of
+                    (case scopes_to_pass_exec funn' func_map b_func_map g_scope_list'''' of
                      | SOME g_scope_list''''' =>
                       (case copyout (MAP FST x_d_l) (MAP SND x_d_l) g_scope_list''''' scope_list' scope_list'' of
                        | SOME (g_scope_list'''''', scope_list''') =>
-                        (case scopes_to_retrieve funn' func_map b_func_map g_scope_list'''' g_scope_list'''''' of
+                        (case scopes_to_retrieve_exec funn' func_map b_func_map g_scope_list'''' g_scope_list'''''' of
                          | SOME g_scope_list''''''' =>
                           SOME (ascope', g_scope_list''''''', ((funn', stmt_stack', scope_list''')::frame_list''), status_running)
                          | _ => NONE)
@@ -2411,7 +2446,7 @@ Definition frames_exec_def:
              | _ => NONE)
            | _ => 
             (* Comp1 *)
-            (case scopes_to_retrieve funn func_map b_func_map g_scope_list g_scope_list'' of
+            (case scopes_to_retrieve_exec funn func_map b_func_map g_scope_list g_scope_list'' of
              | SOME g_scope_list''' =>
               SOME (ascope', g_scope_list''', frame_list'++((funn', stmt_stack', scope_list')::frame_list''), status')
              | _ => NONE))
@@ -2423,7 +2458,7 @@ Definition frames_exec_def:
  (*********)
  (* Comp1, remaining cases *)
  (frames_exec uninit (apply_table_f, ext_map, func_map, b_func_map, pars_map, tbl_map) (ascope, g_scope_list, [(funn, stmt_stack, scope_list)], status_running) =
-  (case scopes_to_pass funn func_map b_func_map g_scope_list of
+  (case scopes_to_pass_exec funn func_map b_func_map g_scope_list of
    | SOME g_scope_list' =>
     (case map_to_pass funn b_func_map of
      | SOME b_func_map' =>
@@ -2431,7 +2466,7 @@ Definition frames_exec_def:
        | SOME tbl_map' =>
         (case stmt_exec uninit (apply_table_f, ext_map, func_map, b_func_map', pars_map, tbl_map') (ascope, g_scope_list', [(funn, stmt_stack, scope_list)], status_running) of
          | SOME (ascope', g_scope_list'', frame_list', status') =>
-          (case scopes_to_retrieve funn func_map b_func_map g_scope_list g_scope_list'' of
+          (case scopes_to_retrieve_exec funn func_map b_func_map g_scope_list g_scope_list'' of
            | SOME g_scope_list''' =>
             SOME (ascope', g_scope_list''', frame_list', status')
            | _ => NONE)
